Finish two-way verified int <-> string conversion

PAC_Checker_LLVM/LLVM_ASCII_String.thy
@@ -261,8 +261,697 @@ lemma ascii_str_int_relD[fcomp_prenorm_simps]:
 
 text \<open>This is overall correctness lemma for our string \<rightarrow> sbi converstion,
   allowing for (partially) verified parsing.\<close>
-context notes [fcomp_norm_unfold] = str_int_assn_def[symmetric] begin
 lemmas str_int_conv_hnr = str_sval_hnr[FCOMP str_sval_id_refine]
+
+section \<open>Conversion from @{typ int} to @{typ string}\<close>
+
+text \<open>Converting an nat to a string is done by simply collecting digits\<close>
+
+fun digits_of_nat :: \<open>nat \<Rightarrow> nat list\<close> where
+  \<open>digits_of_nat n = (if n < 10 then [n] else digits_of_nat (n div 10) @ [n mod 10])\<close>
+
+lemma digits_of_nat_correct: \<open>n = foldl (\<lambda>acc d. 10 * acc + d) 0 (digits_of_nat n)\<close>
+  apply (induction n rule: digits_of_nat.induct)
+  apply (subst digits_of_nat.simps)
+  apply (simp del: digits_of_nat.simps)
+  done
+
+text \<open>The relation between digit and nat is the inverse of @{term char_uval}}\<close>
+
+definition char_of_digit :: \<open>nat \<Rightarrow> char\<close> where
+  \<open>char_of_digit n = char_of (n + 48)\<close>
+
+definition is_digit :: \<open>nat \<Rightarrow> bool\<close> where
+  \<open>is_digit n \<equiv> n < 10\<close>
+
+definition \<open>nat_ascii_char_rel \<equiv> br char_of_digit is_digit\<close>
+
+lemma is_ascii_unum_char_of_digit: \<open>is_digit d \<Longrightarrow> is_ascii_unum (char_of_digit d)\<close>
+  by (auto simp: is_digit_def is_ascii_unum_def char_of_digit_def)
+
+lemma char_uval_char_of_digit: \<open>is_digit d \<Longrightarrow> char_uval (char_of_digit d) = d\<close>
+  by (auto simp: is_digit_def char_uval_def char_of_digit_def)
+
+lemma nat_ascii_char_rel_ascii_char_nat_rel_inv:
+  \<open>nat_ascii_char_rel O ascii_char_nat_rel = Id_on {n. is_digit n}\<close> (is ?A)
+  \<open>ascii_char_nat_rel O nat_ascii_char_rel = Id_on {c. is_ascii_unum c}\<close> (is ?B)
+proof -
+  show ?A
+    unfolding nat_ascii_char_rel_def ascii_char_nat_rel_def
+    by (auto simp: in_br_conv char_of_digit_def is_digit_def char_uval_def is_ascii_unum_def)
+  show ?B
+    unfolding nat_ascii_char_rel_def ascii_char_nat_rel_def
+    by (auto simp: in_br_conv char_of_digit_def is_digit_def char_uval_def is_ascii_unum_def)
+qed
+
+fun chars_of_nat :: \<open>nat \<Rightarrow> string\<close> where
+  \<open>chars_of_nat n = 
+    (if n < 10 then [char_of_digit n] 
+     else chars_of_nat (n div 10) @ [char_of_digit (n mod 10)])\<close>
+
+definition \<open>nat_ascii_str_rel \<equiv> br chars_of_nat (\<lambda>_. True)\<close>
+
+lemma chars_of_nat_neq_Nil[simp]: \<open>chars_of_nat n \<noteq> []\<close>
+  by (subst chars_of_nat.simps) (auto simp del: chars_of_nat.simps)
+
+lemma chars_of_nat_unum[simp]: \<open>\<forall>c \<in> set (chars_of_nat n). is_ascii_unum c\<close>
+  apply (induction n rule: chars_of_nat.induct)
+  apply (subst chars_of_nat.simps)
+  apply (auto simp del: chars_of_nat.simps simp add: is_digit_def
+      intro: is_ascii_unum_char_of_digit)
+  done
+
+lemma str_uval_chars_of_nat[simp]: \<open>str_uval (chars_of_nat n) = n\<close>
+  unfolding str_uval_def
+  apply (induction n rule: chars_of_nat.induct)
+  apply (subst chars_of_nat.simps)
+  apply (auto simp del: chars_of_nat.simps simp add: char_uval_char_of_digit is_digit_def)
+  done
+
+lemma hd_chars_of_nat_not_hyphen[simp]: \<open>hd (chars_of_nat n) \<noteq> ascii_hyphen\<close>
+  by (metis chars_of_nat_neq_Nil chars_of_nat_unum hd_in_set is_ascii_unum_hyphen)
+
+lemma nat_ascii_str_rel_ascii_str_nat_rel_inv:
+  \<open>nat_ascii_str_rel O ascii_str_nat_rel = Id\<close>
+  unfolding nat_ascii_str_rel_def ascii_str_nat_rel_def
+  apply (auto simp: relcomp_unfold is_ascii_unum_str_alt)
+  apply (metis in_br_conv str_uval_chars_of_nat)
+  by (metis chars_of_nat_neq_Nil chars_of_nat_unum in_br_conv 
+            is_ascii_unum_str_alt str_uval_chars_of_nat)
+
+subsubsection \<open>Extending to Integers\<close>
+
+definition chars_of_int :: \<open>int \<Rightarrow> string\<close> where
+  \<open>chars_of_int i \<equiv> 
+    if 0 \<le> i then chars_of_nat (nat i) else ascii_hyphen # chars_of_nat (nat (-i))\<close>
+
+definition \<open>int_ascii_str_rel \<equiv> br chars_of_int (\<lambda>_. True)\<close>
+
+lemma str_sval_chars_of_int[simp]: \<open>str_sval (chars_of_int i) = i\<close>
+  using chars_of_int_def hd_chars_of_nat_not_hyphen str_sval_def str_uval_chars_of_nat 
+  by auto
+
+lemma is_ascii_snum_str_chars_of_int[simp]: \<open>is_ascii_snum_str (chars_of_int i)\<close>
+  by (metis chars_of_int_def chars_of_nat_neq_Nil chars_of_nat_unum 
+            is_ascii_snum_str_def is_ascii_unum_str_alt list.sel(1,3))
+
+lemma int_ascii_str_rel_ascii_str_int_rel_inv:
+  \<open>int_ascii_str_rel O ascii_str_int_rel = Id\<close>
+  unfolding int_ascii_str_rel_def ascii_str_int_rel_def
+  apply (auto simp: relcomp_unfold)
+  apply (metis in_br_conv str_sval_chars_of_int)
+  by (metis in_br_conv is_ascii_snum_str_chars_of_int str_sval_chars_of_int)
+
+subsection \<open>Refinement\<close>
+
+subsubsection \<open>divmod for bigint\<close>
+
+(* this whole subsection essentially just refines the following definition: *)
+definition \<open>divmod_nat \<equiv> \<lambda>(a::nat) (b::nat). (a div b, a mod b)\<close>
+
+definition divmod2by1 :: \<open>limb \<Rightarrow> limb \<Rightarrow> limb \<Rightarrow> (limb \<times> limb) nres\<close> where
+  \<open>divmod2by1 hi lo d \<equiv> doN {
+    ASSERT (0 < unat d \<and> unat hi < unat d);
+    let cur = unat hi * limb_sz + unat lo;
+    RETURN (nat_limb (cur div unat d), nat_limb (cur mod unat d))
+  }\<close>
+
+lemma divmod2by1_spec:
+  assumes \<open>0 < unat d\<close> and \<open>unat hi < unat d\<close>
+  shows \<open>divmod2by1 hi lo d \<le> SPEC (\<lambda>(q, r).
+      unat q = (unat hi * limb_sz + unat lo) div unat d
+    \<and> unat r = (unat hi * limb_sz + unat lo) mod unat d
+    \<and> unat r < unat d)\<close>
+proof -
+  let ?cur = \<open>unat hi * limb_sz + unat lo\<close>
+  have lo_lt: \<open>unat lo < limb_sz\<close> using limb_nat_lt[of lo] unfolding limb_nat_def by simp
+  have d_lt: \<open>unat d < limb_sz\<close> using limb_nat_lt[of d] unfolding limb_nat_def by simp
+  have cur_lt: \<open>?cur < unat d * limb_sz\<close>
+  proof -
+    have \<open>?cur \<le> (unat d - 1) * limb_sz + (limb_sz - 1)\<close>
+      using assms(2) lo_lt by (intro add_mono mult_le_mono) auto
+    also have \<open>\<dots> < unat d * limb_sz\<close>
+      using assms(1) limb_sz_gt(1) by (cases \<open>unat d\<close>) (auto simp: algebra_simps)
+    finally show ?thesis .
+  qed
+  have q_lt: \<open>?cur div unat d < limb_sz\<close>
+    using cur_lt by (simp add: less_mult_imp_div_less mult.commute)
+  have r_lt: \<open>?cur mod unat d < limb_sz\<close>
+    using assms(1) d_lt by (meson mod_less_divisor order_less_trans)
+  show ?thesis
+    unfolding divmod2by1_def
+    apply (refine_vcg)
+    using assms apply simp
+    apply (metis assms(2))
+    using limb_nat_def nat_limb_mod q_lt apply force
+    apply (metis nat_limb_def prod.sel(2) uno_simps(1))
+    by (simp add: nat_limb_def uno_simps(1))
+qed
+
+definition bi_div_by_w64 :: \<open>big_int \<Rightarrow> limb \<Rightarrow> (big_int \<times> limb) nres\<close> where
+  \<open>bi_div_by_w64 bi l \<equiv> doN {
+    ASSERT (0 < unat l);
+    (q, r, _) \<leftarrow> WHILEIT
+      (\<lambda>(q, r, i).
+          i \<le> length bi
+        \<and> length q = length bi
+        \<and> unat r < unat l
+        \<and> unat r = big_int_\<alpha> (drop i bi) mod unat l
+        \<and> big_int_\<alpha> (drop i q) = big_int_\<alpha> (drop i bi) div unat l)
+      (\<lambda>(_, _, i). 0 < i)
+      (\<lambda>(q, r, i). doN {
+        ASSERT (0 < i \<and> i \<le> length bi);
+        (d, r') \<leftarrow> divmod2by1 r (bi ! (i - 1)) l;
+        RETURN (q[i - 1 := d], r', i - 1)
+      })
+      (replicate (length bi) 0, 0, length bi);
+    q \<leftarrow> big_int_trim q;
+    RETURN (q, r)
+  }\<close>
+
+lemma div_step_mod:
+  fixes H d0 l :: nat
+  shows \<open>(d0 + limb_sz * H) mod l = ((H mod l) * limb_sz + d0) mod l\<close>
+  by (metis (no_types, lifting) add.commute mod_add_left_eq mod_mult_right_eq mult.commute)
+
+lemma div_step_div:
+  fixes H d0 l :: nat
+  shows \<open>(d0 + limb_sz * H) div l = (limb_sz * (H div l)) + ((H mod l) * limb_sz + d0) div l\<close>
+proof -
+  have \<open>d0 + limb_sz * H = limb_sz * (H div l) * l + ((H mod l) * limb_sz + d0)\<close>
+    by (metis (full_types) add.commute distrib_left div_mod_decomp
+    group_cancel.add1 mult.commute mult.left_commute)
+  thus ?thesis
+    by (metis Euclidean_Rings.div_eq_0_iff div_mult_self3 mult_0_right
+    nat_arith.rule0)
+qed
+
+lemma div_digit_step:
+  fixes q bi :: big_int and ab :: limb and i l :: nat
+  assumes i_pos: \<open>0 < i\<close> and i_le: \<open>i \<le> length bi\<close> and len_q: \<open>length q = length bi\<close>
+    and inv_q: \<open>big_int_\<alpha> (drop i q) = big_int_\<alpha> (drop i bi) div l\<close>
+    and dig: \<open>unat ab = (big_int_\<alpha> (drop i bi) mod l * limb_sz + unat (bi ! (i - 1))) div l\<close>
+  shows \<open>big_int_\<alpha> (drop (i - 1) (q[i - 1 := ab])) = big_int_\<alpha> (drop (i - 1) bi) div l\<close>
+proof -
+  let ?j = \<open>i - 1\<close>
+  let ?H = \<open>big_int_\<alpha> (drop i bi)\<close>
+  have j_lt_q: \<open>?j < length q\<close> using i_pos i_le len_q by simp
+  have j_lt_bi: \<open>?j < length bi\<close> using i_pos i_le by simp
+  have suc: \<open>Suc ?j = i\<close> using i_pos by simp
+  have drop_q: \<open>drop ?j (q[?j := ab]) = ab # drop i q\<close>
+    using j_lt_q suc
+    by (metis Cons_nth_drop_Suc drop_update_cancel lessI length_list_update
+        nth_list_update_eq)
+  have drop_bi: \<open>drop ?j bi = bi ! ?j # drop i bi\<close>
+    using j_lt_bi suc by (metis Cons_nth_drop_Suc)
+  have \<open>big_int_\<alpha> (drop ?j (q[?j := ab])) = unat ab + limb_sz * (?H div l)\<close>
+    unfolding drop_q using inv_q by (simp add: limb_nat_def)
+  also have \<open>\<dots> = (unat (bi ! ?j) + limb_sz * ?H) div l\<close>
+    using dig by (simp add: div_step_div)
+  also have \<open>\<dots> = big_int_\<alpha> (drop ?j bi) div l\<close>
+    unfolding drop_bi by (simp add: limb_nat_def)
+  finally show ?thesis .
+qed
+
+lemma bi_div_by_w64_correct_aux:
+  assumes bi: \<open>(bi, a::nat) \<in> big_int_rel\<close> and l: \<open>(l, lnn::nat) \<in> unat_rel\<close> and lpos: \<open>0 < lnn\<close>
+  shows \<open>bi_div_by_w64 bi l \<le> \<Down>(big_int_rel \<times>\<^sub>r unat_rel) (RETURN (a div lnn, a mod lnn))\<close>
+proof -
+  have a_eq: \<open>big_int_\<alpha> bi = a\<close> using bi unfolding big_int_rel_def in_br_conv by simp
+  have l_eq: \<open>unat l = lnn\<close>
+    using l unfolding unat_rel_def unat.rel_def in_br_conv by simp
+  show ?thesis
+    unfolding bi_div_by_w64_def
+    apply (refine_vcg
+        WHILEIT_rule[where R=\<open>measure (\<lambda>(_, _, i). i)\<close>
+          and I=\<open>\<lambda>(q, r, i).
+              i \<le> length bi
+            \<and> length q = length bi
+            \<and> unat r < unat l
+            \<and> unat r = big_int_\<alpha> (drop i bi) mod unat l
+            \<and> big_int_\<alpha> (drop i q) = big_int_\<alpha> (drop i bi) div unat l\<close>]
+        divmod2by1_spec
+        big_int_trim_correct)
+    apply simp_all
+    subgoal by (metis lpos l_eq) 
+    subgoal by auto
+    subgoal by auto
+    subgoal by auto
+    subgoal by auto
+    subgoal
+      by (metis Cons_nth_drop_Suc Suc_pred big_int_to_nat.simps(2) div_step_mod
+                limb_nat_def nz_le_conv_less)
+    subgoal
+      apply (clarsimp simp only: One_nat_def[symmetric])
+      apply (rule div_digit_step; assumption)
+      done
+    subgoal
+      by (simp add: a_eq big_int_rel_def brI l_eq unat.rel_def unat_rel_def)
+    done
+qed
+
+lemma bi_div_by_w64_correct:
+  \<open>(uncurry bi_div_by_w64, uncurry (RETURN oo divmod_nat))
+  \<in> [\<lambda>(_, ln). 0 < ln]\<^sub>f big_int_rel \<times>\<^sub>r unat_rel \<rightarrow> \<langle>big_int_rel \<times>\<^sub>r unat_rel\<rangle>nres_rel\<close>
+  apply (intro frefI nres_relI)
+  apply (clarsimp simp: divmod_nat_def)
+  apply (rule bi_div_by_w64_correct_aux; assumption)
+  done
+
+subsubsection \<open>The 128-bit divide-two-by-one primitive\<close>
+
+definition divmod2by1_word :: \<open>limb \<Rightarrow> limb \<Rightarrow> limb \<Rightarrow> (limb \<times> limb)\<close> where
+  \<open>divmod2by1_word hi lo d \<equiv>
+     let cur = (extend hi << limb_wd) + extend lo; dd = extend d
+     in (cutoff (cur div dd), cutoff (cur mod dd))\<close>
+
+lemma extend_unat[simp]: \<open>unat (extend x) = unat x\<close>
+proof -
+  have b: \<open>unat x < 2 ^ LENGTH(double\<^sub>w)\<close>
+    by (rule order_less_le_trans[OF unat_lt2p]) simp
+  show ?thesis
+    by (metis Word.of_nat_unat b unat_of_nat_eq)
+qed
+
+lemma limb_wd_lt_double: \<open>limb_wd < LENGTH(double\<^sub>w)\<close>
+  by (simp add: limb_wd_unfold)
+
+lemma len_double_eq: \<open>(2::nat) ^ LENGTH(double\<^sub>w) = limb_sz * limb_sz\<close>
+  by (metis len_bit0 power_even_eq limb_sz_unfold power2_eq_square)
+
+lemma unat_combine:
+  \<open>unat ((extend hi << limb_wd) + extend lo) = unat hi * limb_sz + unat lo\<close>
+proof -
+  have hi_lt: \<open>unat hi < limb_sz\<close> using limb_nat_lt[of hi] unfolding limb_nat_def by simp
+  have lo_lt: \<open>unat lo < limb_sz\<close> using limb_nat_lt[of lo] unfolding limb_nat_def by simp
+  have sz: \<open>limb_sz = 2 ^ limb_wd\<close> by (simp add: limb_sz_def)
+  have sh: \<open>unat (extend hi << limb_wd) = unat hi * limb_sz\<close>
+  proof -
+    have \<open>unat (extend hi << limb_wd) = (2 ^ limb_wd * unat hi) mod (limb_sz * limb_sz)\<close>
+      by (metis Abs_fnat_hom_mult Word.unat_of_nat len_double_eq shiftl_t2n ucast_nat_def word_unat_power)
+    also have \<open>\<dots> = (unat hi * limb_sz) mod (limb_sz * limb_sz)\<close>
+      by (simp add: sz mult.commute)
+    also have \<open>\<dots> = unat hi * limb_sz\<close>
+      using hi_lt by (simp add: mult_strict_right_mono)
+    finally show ?thesis .
+  qed
+  have sum_lt: \<open>unat hi * limb_sz + unat lo < 2 ^ LENGTH(double\<^sub>w)\<close>
+    using hi_lt lo_lt unfolding len_double_eq
+    by (metis hi_lt lo_lt mlex_bound)
+  show ?thesis
+    using sum_lt sh unat_add_lem[of \<open>extend hi << limb_wd\<close> \<open>extend lo\<close>]
+    by simp
+qed
+
+lemma divmod2by1_word_eq:
+  \<open>divmod2by1_word hi lo d =
+     (nat_limb ((unat hi * limb_sz + unat lo) div unat d),
+      nat_limb ((unat hi * limb_sz + unat lo) mod unat d))\<close>
+  unfolding divmod2by1_word_def Let_def cutoff_limb
+  by (simp add: unat_div unat_mod unat_combine)
+
+lemma divmod2by1_word_refine:
+  \<open>(uncurry2 (RETURN ooo divmod2by1_word), uncurry2 divmod2by1)
+   \<in> (Id \<times>\<^sub>r Id) \<times>\<^sub>r Id \<rightarrow>\<^sub>f \<langle>Id\<rangle>nres_rel\<close>
+  apply (intro frefI nres_relI; clarsimp simp: divmod2by1_def)
+  apply refine_vcg
+  apply (simp add: divmod2by1_word_eq)
+  by (meson order_mono_setup.refl)
+
+sepref_register divmod2by1
+
+lemma extend_neq_zero[simp]: \<open>extend d \<noteq> 0 \<longleftrightarrow> d \<noteq> 0\<close>
+  by (metis extend_unat unat_eq_zero)
+
+sepref_def divmod2by1_impl is \<open>uncurry2 (RETURN ooo divmod2by1_word)\<close>
+  :: \<open>[\<lambda>((hi, lo), d). d \<noteq> 0]\<^sub>a limb_assn\<^sup>k *\<^sub>a limb_assn\<^sup>k *\<^sub>a limb_assn\<^sup>k \<rightarrow> limb_assn \<times>\<^sub>a limb_assn\<close>
+  unfolding divmod2by1_word_def
+  supply [simp] = is_upcast limb_wd_unfold
+  apply (rewrite at "_ << \<hole>" annot_snat_snat_upcast[where 'l="double\<^sub>w"])
+  by sepref
+
+lemmas divmod2by1_hnr[sepref_fr_rules] = divmod2by1_impl.refine[FCOMP divmod2by1_word_refine]
+
+subsubsection \<open>The long-division loop\<close>
+
+sepref_register bi_div_by_w64
+
+sepref_def bi_div_by_w64_impl is \<open>uncurry bi_div_by_w64\<close>
+  :: \<open>bi_aux_assn\<^sup>k *\<^sub>a limb_assn\<^sup>k \<rightarrow>\<^sub>a bi_aux_assn \<times>\<^sub>a limb_assn\<close>
+  unfolding bi_div_by_w64_def
+  apply (annot_snat_const size_t)
+  apply (rewrite al_fold_custom_replicate)
+  by sepref
+
+context notes [fcomp_norm_unfold] = bi_assn_def[symmetric]
+begin
+lemmas bi_div_by_w64_hnr[sepref_fr_rules] =
+  bi_div_by_w64_impl.refine[FCOMP bi_div_by_w64_correct]
+end
+
+subsubsection \<open>Unsigned Bigint to nat\<close>
+
+text \<open>We can define @{term chars_of_nat} imperatively, using nat.\<close>
+
+definition chars_of_nat_nres :: \<open>nat \<Rightarrow> string nres\<close> where
+  \<open>chars_of_nat_nres n \<equiv> doN {
+    (cs,r) \<leftarrow> WHILEIT
+      (\<lambda>(cs,m). chars_of_nat n = chars_of_nat m @ cs)
+      (\<lambda>(cs,n). 9 < n)
+      (\<lambda>(cs,n). doN {
+        let (q,r) = divmod_nat n 10;
+        ASSERT(r < 10);
+        RETURN ((char_of_digit r)#cs,q)
+      }) ([], n);
+    ASSERT (r < 10);
+    RETURN ((char_of_digit r)#cs)
+  }\<close>
+
+lemma chars_of_nat_base: \<open>m < 10 \<Longrightarrow> chars_of_nat m = [char_of_digit m]\<close>
+  by (subst chars_of_nat.simps) simp
+
+lemma chars_of_nat_step:
+  \<open>\<not> m < 10 \<Longrightarrow> chars_of_nat m = chars_of_nat (m div 10) @ [char_of_digit (m mod 10)]\<close>
+  by (subst chars_of_nat.simps) simp
+
+lemma char_of_nat_refine: \<open>chars_of_nat_nres n \<le> SPEC (\<lambda>cs. cs = (chars_of_nat n))\<close>
+  unfolding chars_of_nat_nres_def divmod_nat_def
+  apply (refine_vcg WHILEIT_rule[where R=\<open>measure (\<lambda>(_, m). m)\<close>])
+  apply (auto simp del: chars_of_nat.simps simp add: chars_of_nat_base chars_of_nat_step)
+  done
+
+lemma char_of_nat_href_spec:
+  \<open>(chars_of_nat_nres, RETURN o chars_of_nat) 
+    \<in> Id \<rightarrow>\<^sub>f \<langle>Id\<rangle>nres_rel\<close>
+  apply (intro frefI nres_relI)
+  by (smt (verit, del_insts) Id_refine char_of_nat_refine inres_simps(2) mem_Collect_eq 
+    nofail_simps(2) nres_order_simps(21) pair_in_Id_conv push_in_let_conv(2) pw_le_iff)
+
+definition char_of_digit_sbi :: \<open>big_int \<Rightarrow> char\<close> where
+  \<open>char_of_digit_sbi sbi \<equiv> char_of (unat (get_or_zero sbi 0) + 48)\<close>
+
+lemma char_of_digit_sbi_spec:
+  \<open>(char_of_digit_sbi, char_of_digit) \<in> [is_digit]\<^sub>f big_int_rel \<rightarrow> Id\<close>
+proof (intro frefI)
+  fix sbi :: big_int and n :: nat
+  assume dig: \<open>is_digit n\<close> and rel: \<open>(sbi, n) \<in> big_int_rel\<close>
+  have inv: \<open>big_int_invar sbi\<close> and n_eq: \<open>n = big_int_\<alpha> sbi\<close>
+    using rel by (auto simp: big_int_rel_def in_br_conv)
+  have \<open>char_of_digit_sbi sbi = char_of_digit n\<close>
+  proof (cases sbi)
+    case Nil
+    then show ?thesis
+      using n_eq by (simp add: char_of_digit_sbi_def char_of_digit_def get_or_zero_def)
+  next
+    case (Cons x xs)
+    have \<open>big_int_\<alpha> xs = 0\<close>
+    proof (rule ccontr)
+      assume \<open>big_int_\<alpha> xs \<noteq> 0\<close>
+      hence \<open>limb_sz \<le> limb_sz * big_int_\<alpha> xs\<close>
+        using mult_le_mono2[of 1 \<open>big_int_\<alpha> xs\<close> limb_sz] by simp
+      moreover have \<open>limb_sz * big_int_\<alpha> xs \<le> n\<close>
+        using n_eq Cons by simp
+      moreover have \<open>(10::nat) \<le> limb_sz\<close>
+        by (simp add: limb_sz_unfold)
+      ultimately show False
+        using dig
+        by (meson is_digit_def le_trans linorder_not_le)
+    qed
+    then obtain k where k: \<open>xs = replicate k 0\<close>
+      using big_int_to_nat_0 by auto
+    have \<open>xs = []\<close>
+    proof (rule ccontr)
+      assume ne: \<open>xs \<noteq> []\<close>
+      hence \<open>last xs = 0\<close>
+        using k by (metis in_set_replicate last_in_set)
+      moreover have \<open>last (x # xs) \<noteq> 0\<close>
+        using inv Cons by (simp add: big_int_invar_def)
+      ultimately show False
+        using ne by simp
+    qed
+    then show ?thesis
+      using n_eq Cons
+      by (simp add: char_of_digit_sbi_def char_of_digit_def get_or_zero_def limb_nat_def)
+  qed
+  thus \<open>(char_of_digit_sbi sbi, char_of_digit n) \<in> Id\<close> by simp
+qed
+
+subsubsection \<open>LLVM implementation of the digit-to-char conversion\<close>
+
+definition cutoff8 :: \<open>limb \<Rightarrow> 8 word\<close> where
+  \<open>cutoff8 w \<equiv> UCAST(limb\<^sub>w \<rightarrow> 8) w\<close>
+
+sepref_register cutoff8
+
+context begin
+interpretation llvm_prim_arith_setup .
+lemma cutoff8_hnr[sepref_fr_rules]:
+  \<open>(\<lambda>w. ll_trunc w TYPE(8 word), RETURN o cutoff8) \<in> limb_assn\<^sup>k \<rightarrow>\<^sub>a word_assn' TYPE(8)\<close>
+  unfolding cutoff8_def
+  supply [simp] = is_down'
+  apply sepref_to_hoare
+  by vcg
+end
+
+definition char_of_digit_limb :: \<open>limb \<Rightarrow> char\<close> where
+  \<open>char_of_digit_limb x \<equiv> char_of (unat x + 48)\<close>
+
+lemma char_of_digit_limb_alt:
+  \<open>char_of_digit_limb x = char_of_word (cutoff8 (x + 48))\<close>
+proof -
+  have dvd1: \<open>(2::nat) ^ 8 dvd 2 ^ 64\<close>
+    by (rule le_imp_power_dvd) simp
+  hence dvd2: \<open>(256::nat) dvd 2 ^ 64\<close>
+    by simp
+  have dvd3: \<open>(256::nat) dvd 18446744073709551616\<close>
+    by eval
+  show ?thesis
+    unfolding char_of_digit_limb_def char_of_word_def cutoff8_def
+    by (simp add: unat_ucast unat_word_ariths
+        mod_mod_cancel[OF dvd1] mod_mod_cancel[OF dvd2] mod_mod_cancel[OF dvd3])
+qed
+
+sepref_register char_of_digit_limb
+
+sepref_def char_of_digit_limb_impl [llvm_inline] is \<open>RETURN o char_of_digit_limb\<close>
+  :: \<open>limb_assn\<^sup>k \<rightarrow>\<^sub>a char_assn\<close>
+  unfolding char_of_digit_limb_alt
+  by sepref
+
+definition char_of_digit_sbi_nres :: \<open>big_int \<Rightarrow> char nres\<close> where
+  \<open>char_of_digit_sbi_nres sbi \<equiv> doN {
+     if length sbi = 0 then RETURN (char_of_digit_limb 0)
+     else doN { x \<leftarrow> mop_list_get sbi 0; RETURN (char_of_digit_limb x) }
+   }\<close>
+
+lemma char_of_digit_sbi_nres_correct:
+  assumes dig: \<open>is_digit n\<close> and rel: \<open>(sbi, n) \<in> big_int_rel\<close>
+  shows \<open>char_of_digit_sbi_nres sbi \<le> RETURN (char_of_digit n)\<close>
+proof -
+  have eq: \<open>char_of_digit_sbi sbi = char_of_digit n\<close>
+    using char_of_digit_sbi_spec dig rel by (auto simp: fref_def)
+  show ?thesis
+    using eq
+    by (auto simp: char_of_digit_sbi_nres_def char_of_digit_sbi_def char_of_digit_limb_def
+        get_or_zero_def pw_le_iff refine_pw_simps)
+qed
+
+lemma char_of_digit_sbi_nres_spec:
+  \<open>(char_of_digit_sbi_nres, RETURN o char_of_digit) \<in> [is_digit]\<^sub>f big_int_rel \<rightarrow> \<langle>Id\<rangle>nres_rel\<close>
+  by (intro frefI nres_relI) (auto simp: char_of_digit_sbi_nres_correct)
+
+context notes [fcomp_norm_unfold] = bi_assn_def[symmetric] begin
+
+sepref_def char_of_digit_sbi_impl is \<open>char_of_digit_sbi_nres\<close>
+  :: \<open>bi_aux_assn\<^sup>k \<rightarrow>\<^sub>a char_assn\<close>
+  unfolding char_of_digit_sbi_nres_def
+  apply (annot_snat_const size_t)
+  by sepref
+
+lemmas char_of_digit_hnr[sepref_fr_rules] =
+  char_of_digit_sbi_impl.refine[FCOMP char_of_digit_sbi_nres_spec]
+
+definition \<open>gt_nine \<equiv> \<lambda>(n::nat). 9 < n\<close>
+
+lemma gt_nine_fold: \<open>(9 < n) = gt_nine n\<close>
+  by (simp add: gt_nine_def)
+
+sepref_register gt_nine
+
+definition gt_nine_bi_nres :: \<open>big_int \<Rightarrow> bool nres\<close> where
+  \<open>gt_nine_bi_nres bi \<equiv> doN {
+     if 1 < length bi then RETURN True
+     else if length bi = 0 then RETURN False
+     else doN { x \<leftarrow> mop_list_get bi 0; RETURN ((9::limb) < x) }
+   }\<close>
+
+lemma gt_nine_bi_nres_correct:
+  assumes rel: \<open>(bi, n) \<in> big_int_rel\<close>
+  shows \<open>gt_nine_bi_nres bi \<le> RETURN (gt_nine n)\<close>
+proof -
+  have inv: \<open>big_int_invar bi\<close> and n_eq: \<open>n = big_int_\<alpha> bi\<close>
+    using rel by (auto simp: big_int_rel_def in_br_conv)
+  show ?thesis
+  proof (cases bi)
+    case Nil
+    then show ?thesis
+      using n_eq by (simp add: gt_nine_bi_nres_def gt_nine_def)
+  next
+    case bi_cons: (Cons x xs)
+    show ?thesis
+    proof (cases xs)
+      case Nil
+      hence bi_eq: \<open>bi = [x]\<close>
+        using bi_cons by simp
+      hence n_val: \<open>n = unat x\<close>
+        using n_eq by (simp add: limb_nat_def)
+      show ?thesis
+        by (auto simp: gt_nine_bi_nres_def gt_nine_def bi_eq n_val word_less_nat_alt
+            pw_le_iff refine_pw_simps)
+    next
+      case cons2: (Cons y ys)
+      hence len: \<open>1 < length bi\<close>
+        using bi_cons by simp
+      have \<open>n \<noteq> 0\<close>
+      proof
+        assume \<open>n = 0\<close>
+        then obtain k where k: \<open>bi = replicate k 0\<close>
+          using n_eq big_int_to_nat_0 by auto
+        have ne: \<open>bi \<noteq> []\<close>
+          using len by auto
+        hence \<open>last bi \<noteq> 0\<close>
+          using inv by (simp add: big_int_invar_def)
+        moreover have \<open>last bi = 0\<close>
+          using k ne by (metis in_set_replicate last_in_set)
+        ultimately show False by simp
+      qed
+      hence lb: \<open>limb_sz ^ (length bi - 1) \<le> n\<close>
+        using big_int_rel_bounds(2)[OF rel] by simp
+      have \<open>limb_sz ^ 1 \<le> limb_sz ^ (length bi - 1)\<close>
+        by (rule power_increasing) (use len limb_sz_gt(1) in auto)
+      hence \<open>limb_sz \<le> limb_sz ^ (length bi - 1)\<close>
+        by simp
+      moreover have \<open>(9::nat) < limb_sz\<close>
+        by (simp add: limb_sz_unfold)
+      ultimately have \<open>gt_nine n\<close>
+        using lb unfolding gt_nine_def by linarith
+      then show ?thesis
+        using len by (simp add: gt_nine_bi_nres_def)
+    qed
+  qed
+qed
+
+lemma gt_nine_bi_nres_spec:
+  \<open>(gt_nine_bi_nres, RETURN o gt_nine) \<in> big_int_rel \<rightarrow>\<^sub>f \<langle>bool_rel\<rangle>nres_rel\<close>
+  by (intro frefI nres_relI) (auto simp: gt_nine_bi_nres_correct)
+
+sepref_def gt_nine_bi_impl is \<open>gt_nine_bi_nres\<close>
+  :: \<open>bi_aux_assn\<^sup>k \<rightarrow>\<^sub>a bool1_assn\<close>
+  unfolding gt_nine_bi_nres_def
+  apply (annot_snat_const size_t)
+  by sepref
+
+lemmas gt_nine_hnr[sepref_fr_rules] =
+  gt_nine_bi_impl.refine[FCOMP gt_nine_bi_nres_spec]
+
+lemma char_of_digit_limb_unat_refine:
+  \<open>(RETURN o char_of_digit_limb, RETURN o char_of_digit) \<in> unat_rel \<rightarrow>\<^sub>f \<langle>Id\<rangle>nres_rel\<close>
+  by (intro frefI nres_relI)
+     (auto simp: char_of_digit_limb_def char_of_digit_def unat_rel_def unat.rel_def
+       in_br_conv)
+
+lemmas char_of_digit_unat_hnr[sepref_fr_rules] =
+  char_of_digit_limb_impl.refine[FCOMP char_of_digit_limb_unat_refine]
+
+sepref_register char_of_digit
+sepref_def char_of_nat_impl is \<open>chars_of_nat_nres\<close>
+  :: \<open>bi_assn\<^sup>d \<rightarrow>\<^sub>a strl_assn'\<close>
+  unfolding chars_of_nat_nres_def gt_nine_fold
+  supply [simp] = is_digit_def
+  apply (annot_unat_const size_t)
+  by sepref
+
+lemmas char_of_nat_hnr[sepref_fr_rules] = 
+  char_of_nat_impl.refine[FCOMP char_of_nat_href_spec]
+
+subsubsection \<open>Extending to signed big integers\<close>
+
+definition \<open>int_sign \<equiv> \<lambda>(i::int). if i < 0 then True else False\<close>
+
+lemma int_sign_impl[sepref_fr_rules]:
+  \<open>(\<lambda>(sbi,s). Mreturn s, RETURN o int_sign)
+  \<in> sbi_assn\<^sup>k \<rightarrow>\<^sub>a bool1_assn\<close>
+  unfolding int_sign_def
+  apply sepref_to_hoare
+  apply vcg
+  apply (auto simp: ENTAILS_def entails_def sep_algebra_simps
+    bool1_rel_def bool.rel_def in_br_conv sbi_assn_def pure_def
+    hr_comp_def signed_big_int_rel_def signed_big_int_to_int_def
+    signed_big_int_invar_def \<sigma>_def)
+  using big_int_to_nat_not0 apply blast
+  using big_int_to_nat_not0 apply blast
+  using big_int_to_nat_not0 by blast
+
+definition \<open>int_abs_nat \<equiv> nat o abs\<close>
+
+lemma limbs_of_sbi_impl[sepref_fr_rules]:
+  \<open>(\<lambda>(sbi,s).Mreturn sbi, RETURN o int_abs_nat)
+  \<in> sbi_assn\<^sup>d \<rightarrow>\<^sub>a bi_assn\<close>
+  unfolding int_abs_nat_def
+  apply (sepref_to_hoare; vcg)
+  apply (auto simp: ENTAILS_def entails_def sep_algebra_simps
+  sbi_assn_def bi_assn_def hr_comp_def bool1_rel_def pure_def
+  bool.rel_def in_br_conv signed_big_int_rel_def 
+  signed_big_int_to_int_def signed_big_int_invar_def big_int_rel_def)
+  using limbs_of_def apply force
+  using big_int_invar_def limbs_of_def apply auto[1]
+  apply (metis big_int_invar_def fst_conv limbs_of_def)
+  using big_int_to_nat_not0 by blast
+
+definition chars_of_int_nres :: \<open>int \<Rightarrow> string nres\<close> where
+  \<open>chars_of_int_nres i \<equiv> doN {
+    let \<sigma> = int_sign i;
+    if \<sigma> then doN {
+      let n = int_abs_nat i;
+      let csn = chars_of_nat n;
+      RETURN (ascii_hyphen#csn)
+    } else doN {
+      let n = int_abs_nat i;
+      let csn = chars_of_nat n;
+      RETURN (csn)
+    }
+  }\<close>
+
+lemma char_of_int_spec:
+  \<open>(chars_of_int_nres, RETURN o chars_of_int)
+  \<in> Id \<rightarrow>\<^sub>f \<langle>Id\<rangle>nres_rel\<close>
+  apply (intro frefI nres_relI)
+  unfolding chars_of_int_nres_def chars_of_int_def
+    int_sign_def int_abs_nat_def
+  by (smt (verit, del_insts) Id_refine comp_apply pair_in_Id_conv)
+  
+sepref_def chars_of_int_impl is \<open>chars_of_int_nres\<close>
+  :: \<open>sbi_assn\<^sup>d \<rightarrow>\<^sub>a strl_assn'\<close>
+  unfolding chars_of_int_nres_def
+  by sepref
+
+lemmas chars_of_int_hnr[sepref_fr_rules] =
+  chars_of_int_impl.refine[FCOMP char_of_int_spec]
+
+text \<open>We can compose with the high level ascii semantics like we did 
+  for string \<rightarrow> int\<close>
+
+definition sbi_str_assn where
+  \<open>sbi_str_assn \<equiv> hr_comp sbi_assn int_ascii_str_rel\<close>
+
+lemma chars_of_int_id_refine:
+  \<open>(RETURN o chars_of_int, RETURN o id)
+  \<in> int_ascii_str_rel \<rightarrow>\<^sub>f \<langle>Id\<rangle>nres_rel\<close>
+  by (intro frefI nres_relI) (auto simp: int_ascii_str_rel_def in_br_conv)
+
+text \<open>This is overall correctness lemma for our sbi \<rightarrow> string converstion\<close>
+lemmas int_str_conv_hnr = chars_of_int_hnr[FCOMP chars_of_int_id_refine]
+
 end
 
 end
